This test involves some assumptions about the positive sequence.

Given a series $\sum\limits_{n=0}^{\infty}(-1)^{n}a_n$ 

If the following 3 requirements are met:

1. $a_n$ is positive for $n\ge0$
2. $a_n$ is decreasing for $n\ge0$
3. $a_n$ converges to 0 ($\lim_{n\to \infty}a_n=0$)

Then the series $\sum\limits_{n=0}^{\infty}(-1)^{n}a_n$ *converges* 
**Warning**: 
This test only determines convergence, but not whether it is *absolutely* or *conditionally* convergent.

If the requirements are not met the test is *inconclusive*.